wip

Std/Data/HashMap/Lemmas.lean
@@ -80,9 +80,10 @@ theorem Array.exists_get_of_mem_data {as : Array α} {a : α}
     | inr h => exact ih h
 
 namespace Std.HashMap
-open List
-
 variable [BEq α] [Hashable α] [LawfulHashable α] [PartialEquivBEq α]
+
+namespace Imp
+open List
 
 -- NOTE(WN): These would ideally be solved by a congruence-closure-for-PERs tactic
 -- See https://leanprover.zulipchat.com/#narrow/stream/270676-lean4/topic/Rewriting.20congruent.20relations
@@ -93,49 +94,64 @@ private theorem beq_nonsense_1 {a b c : α} : a != b → a == c → b != c :=
 private theorem beq_nonsense_2 {a b c : α} : a == b → b == c → ¬(c != a) :=
   fun h₁ h₂ h₃ => Bool.bne_iff_not_beq.mp (bne_symm h₃) (PartialEquivBEq.trans h₁ h₂)
 
-/-- It is a bit easier to reason about `foldl (append)` than `foldl (foldl)`, so we use this
-(less efficient) variant of `toList` as the mathematical model. -/
-def toListModel (m : HashMap α β) : List (α × β) :=
-  m.val.buckets.val.foldl (init := []) (fun acc bkt => acc ++ bkt.toList)
-
-theorem toList_eq_reverse_toListModel (m : HashMap α β) : m.toList = m.toListModel.reverse := by
-  simp only [toList, toListModel, fold, Imp.fold, Array.foldl_eq_foldl_data, AssocList.foldl_eq,
-    List.foldl_cons_fn]
-  suffices ∀ (l₁ : List (AssocList α β)) (l₂ : List (α × β)),
-      l₁.foldl (init := l₂.reverse) (fun d b => b.toList.reverse ++ d) =
-      (l₁.foldl (init := l₂) fun acc bkt => acc ++ bkt.toList).reverse by
-    apply this (l₂ := [])
-  intro l₁
-  induction l₁ with
-  | nil => intro; rfl
-  | cons a as ih =>
-    intro l₂
-    simp only [List.foldl, ← List.reverse_append, ih]
+namespace Buckets
 
 /-- The contents of any given bucket are pairwise `bne`. -/
-theorem Pairwise_bne_bucket (m : HashMap α β) (i : Fin m.val.buckets.val.size) :
-  Pairwise (·.1 != ·.1) m.val.buckets.val[i].toList := by
-  have hWF := Imp.WF_iff.mp m.property |>.right
-  have := hWF.distinct m.val.buckets.val[i] (Array.getElem_mem_data _ _)
+theorem Pairwise_bne_bucket (bkts : Buckets α β) (H : bkts.WF) (i : Nat) (h : i < bkts.val.size)
+  : Pairwise (·.1 != ·.1) bkts.val[i].toList := by
+  have := H.distinct bkts.val[i] (Array.getElem_mem_data _ _)
   exact List.Pairwise.imp Bool.bne_iff_not_beq.mpr this
 
+/-- Reformulation of `Pairwise_bne_bucket` for use with `List.foo_of_unique`. -/
+theorem Pairwise_bne_bucket' (bkts : Buckets α β) (H : bkts.WF) (i : Nat)
+    (h : i < bkts.val.size) (a : α)
+    : Pairwise (fun p q => p.1 == a → q.1 != a) bkts.val[i].toList :=
+  List.Pairwise.imp beq_nonsense_1 (Pairwise_bne_bucket bkts H i h)
+
+/-- It is a bit easier to reason about `foldl (append)` than `foldl (foldl)`, so we use this
+(less efficient) variant of `toList` as the mathematical model. -/
+def toListModel (bkts : Buckets α β) : List (α × β) :=
+  -- Note(WN): the implementation is  `bkts.foldl` rather than `bkts.data.foldl` because we need
+  -- to reason about array indices in some of the theorems.
+  bkts.val.foldl (init := []) (fun acc bkt => acc ++ bkt.toList)
+
+theorem mem_toListModel_iff_mem_bucket (bkts : Buckets α β) (H : bkts.WF) (a : α) (b : β)
+    : haveI := mkIdx bkts.property a
+      (a, b) ∈ bkts.toListModel ↔ (a, b) ∈ (bkts.val[this.1]'this.2).toList := by
+  have : (a, b) ∈ bkts.toListModel ↔ ∃ bkt ∈ bkts.val.data, (a, b) ∈ bkt.toList := by
+    simp [toListModel, Array.foldl_eq_foldl_data, List.foldl_append_fn, List.nil_append,
+      List.mem_bind]
+  rw [this]
+  clear this
+  apply Iff.intro
+  . intro ⟨bkt, hBkt, hMem⟩
+    have ⟨i, hGetI⟩ := Array.exists_get_of_mem_data hBkt
+    simp only [getElem_fin] at hGetI
+    suffices (mkIdx bkts.property a).val.toNat = i by
+      simp [Array.ugetElem_eq_getElem, this, ← hGetI, hMem]
+    unfold Imp.mkIdx
+    dsimp
+    exact H.hash_self i.val i.isLt (a, b) (hGetI ▸ hMem)
+  . intro h
+    refine ⟨_, Array.getElem_mem_data _ _, h⟩
+
 /-- The map does not store duplicate (by `beq`) keys. -/
-theorem Pairwise_bne_toListModel (m : HashMap α β) : m.toListModel.Pairwise (·.1 != ·.1) := by
+theorem Pairwise_bne_toListModel (bkts : Buckets α β) (H : bkts.WF)
+    : bkts.toListModel.Pairwise (·.1 != ·.1) := by
   unfold toListModel
   refine Array.foldl_induction
     (motive := fun i (acc : List (α × β)) =>
       -- The acc has the desired property
       acc.Pairwise (·.1 != ·.1)
       -- All not-yet-accumulated buckets are pairwise disjoint with the acc
-      ∧ ∀ j, i ≤ j → (_ : j < m.val.buckets.val.size) →
-        ∀ p ∈ acc, ∀ r ∈ m.val.buckets.val[j].toList, p.1 != r.1)
+      ∧ ∀ j, i ≤ j → (_ : j < bkts.val.size) →
+        ∀ p ∈ acc, ∀ r ∈ bkts.val[j].toList, p.1 != r.1)
     ?h0 ?hf |>.left
   case h0 => exact ⟨List.Pairwise.nil, fun.⟩
   case hf =>
-    have hWF := Imp.WF_iff.mp m.property |>.right
     intro i acc h
     refine ⟨List.pairwise_append.mpr ⟨h.left, ?bkt, ?accbkt⟩, ?accbkts⟩
-    case bkt => apply Pairwise_bne_bucket
+    case bkt => apply Pairwise_bne_bucket bkts H
     case accbkt =>
       intro a hA b hB
       exact h.right i.val (Nat.le_refl _) i.isLt a hA b hB
@@ -148,78 +164,97 @@ theorem Pairwise_bne_toListModel (m : HashMap α β) : m.toListModel.Pairwise (�
         refine Bool.bne_iff_not_beq.mpr fun h => ?_
         have hHashEq := LawfulHashable.hash_eq h
         have hGt := Nat.lt_of_succ_le hGe
-        have hHashP := hWF.hash_self i (Nat.lt_trans hGt hLt) _ hP
-        have hHashR := hWF.hash_self j hLt _ hR
+        have hHashP := H.hash_self i (Nat.lt_trans hGt hLt) _ hP
+        have hHashR := H.hash_self j hLt _ hR
         dsimp at hHashP hHashR
         have : i.val = j := by
           rw [hHashEq] at hHashP
           exact .trans hHashP.symm hHashR
         exact Nat.ne_of_lt hGt this
 
+/-- Reformulation of `Pairwise_bne_toListModel` for use with `List.foo_of_unique`. -/
+theorem Pairwise_bne_toListModel' (bkts : Buckets α β) (H : bkts.WF) (a : α)
+    : bkts.toListModel.Pairwise (fun p q => p.1 == a → q.1 != a) :=
+  List.Pairwise.imp beq_nonsense_1 (Pairwise_bne_toListModel bkts H)
+
+theorem toListModel_expand (size : Nat) (bkts : Buckets α β)
+    : (expand size bkts).buckets.toListModel ~ bkts.toListModel :=
+  sorry
+
+end Buckets
+
+theorem findEntry?_eq (m : Imp α β) (H : m.WF) (a : α)
+    : m.findEntry? a = m.buckets.toListModel.find? (·.1 == a) := by
+  have hWf := WF_iff.mp H |>.right
+  have hPairwiseBkt :
+      haveI := mkIdx m.buckets.property a
+      Pairwise (fun p q => p.1 == a → q.1 != a) (m.buckets.val[this.1]'this.2).toList :=
+    by apply Buckets.Pairwise_bne_bucket' m.buckets hWf
+  apply Option.ext
+  intro (a', b)
+  simp only [Option.mem_def, findEntry?, Imp.findEntry?, AssocList.findEntry?_eq,
+    List.find?_eq_some_of_unique (Buckets.Pairwise_bne_toListModel' m.buckets hWf a),
+    List.find?_eq_some_of_unique hPairwiseBkt,
+    and_congr_left_iff]
+  intro hBeq
+  have : hash a' = hash a := LawfulHashable.hash_eq hBeq
+  simp [Buckets.mem_toListModel_iff_mem_bucket m.buckets hWf, mkIdx, this]
+
+theorem toListModel_insert_perm_cons_eraseP (m : Imp α β) (H : m.WF) (a : α) (b : β)
+    : (m.insert a b).buckets.toListModel ~ (a, b) :: m.buckets.toListModel.eraseP (·.1 == a) := by
+  dsimp [insert, cond]
+  split
+  -- By foldl_induction probably:
+  -- `insert a` leaves all the non-a buckets alone
+  -- this same lemma but holds of the bucket at `a`
+  -- and then when things get resized, apply `toListModel_expand`
+  sorry
+  sorry
+
+theorem toListModel_erase_eq_eraseP (m : Imp α β) (H : m.WF) (a : α)
+    : (m.erase a).buckets.toListModel = m.buckets.toListModel.eraseP (·.1 == a) :=
+  sorry
+
+end Imp
+
+theorem toList_eq_reverse_toListModel (m : HashMap α β)
+    : m.toList = m.val.buckets.toListModel.reverse := by
+  simp only [toList, Imp.Buckets.toListModel, fold, Imp.fold, Array.foldl_eq_foldl_data,
+    AssocList.foldl_eq, List.foldl_cons_fn]
+  suffices ∀ (l₁ : List (AssocList α β)) (l₂ : List (α × β)),
+      l₁.foldl (init := l₂.reverse) (fun d b => b.toList.reverse ++ d) =
+      (l₁.foldl (init := l₂) fun acc bkt => acc ++ bkt.toList).reverse by
+    apply this (l₂ := [])
+  intro l₁
+  induction l₁ with
+  | nil => intro; rfl
+  | cons a as ih =>
+    intro l₂
+    simp only [List.foldl, ← List.reverse_append, ih]
+
+-- TODO: sort below later
+#exit
+
 theorem toListModel_eraseP_eq_toListModel_filter (m : HashMap α β)
-    : m.toListModel.eraseP (·.1 == a) = m.toListModel.filter (·.1 != a) := by
+    : m.val.buckets.toListModel.eraseP (·.1 == a) = m.val.buckets.toListModel.filter (·.1 != a) :=
+  by
   apply List.eraseP_eq_filter_of_unique
   apply List.Pairwise.imp ?_ (Pairwise_bne_toListModel _)
   intro (a₁, _) (a₂, _) hA₁Bne hA₁Beq
   rw [Bool.not_eq_true_iff_ne_true, ← Bool.bne_iff_not_beq]
   exact beq_nonsense_1 hA₁Bne hA₁Beq
 
-theorem mem_toListModel_iff_mem_bucket (m : HashMap α β) (a : α) (b : β)
-    : haveI := Imp.mkIdx m.val.buckets.2 a
-      (a, b) ∈ m.toListModel ↔ (a, b) ∈ (m.val.buckets.val[this.1]'this.2).toList := by
-  have : (a, b) ∈ m.toListModel ↔ ∃ bkt ∈ m.val.buckets.val.data, (a, b) ∈ bkt.toList := by
-    simp [toListModel, Array.foldl_eq_foldl_data, List.foldl_append_fn, List.nil_append,
-      List.mem_bind]
-  rw [this]
-  clear this
-  apply Iff.intro
-  . intro ⟨bkt, hBkt, hMem⟩
-    have ⟨i, hGetI⟩ := Array.exists_get_of_mem_data hBkt
-    simp only [getElem_fin] at hGetI
-    suffices (Imp.mkIdx m.val.buckets.2 a).val.toNat = i by
-      simp [Array.ugetElem_eq_getElem, this, ← hGetI, hMem]
-    unfold Imp.mkIdx
-    dsimp
-    exact Imp.WF_iff.mp m.property |>.right |>.hash_self i.val i.isLt (a, b) (hGetI ▸ hMem)
-  . intro h
-    refine ⟨_, Array.getElem_mem_data _ _, h⟩
-
-theorem findEntry?_eq (m : HashMap α β) (a : α)
-    : m.findEntry? a = m.toListModel.find? (·.1 == a) := by
-  have hPairwiseM : Pairwise (fun p q => p.1 == a → q.1 != a) m.toListModel :=
-    Pairwise.imp (fun p q => beq_nonsense_1 p q) (Pairwise_bne_toListModel m)
-  have hPairwiseBkt :
-      haveI := Imp.mkIdx m.val.buckets.property a
-      Pairwise (fun p q => p.1 == a → q.1 != a) (m.val.buckets.val[this.1]'this.2).toList := by
-    sorry
-  apply Option.ext
-  intro (a', b)
-  simp only [Option.mem_def, findEntry?, Imp.findEntry?, AssocList.findEntry?_eq,
-    List.find?_eq_some_of_unique hPairwiseM, List.find?_eq_some_of_unique hPairwiseBkt,
-    and_congr_left_iff]
-  intro hBeq
-  have : hash a' = hash a := LawfulHashable.hash_eq hBeq
-  simp [mem_toListModel_iff_mem_bucket, Imp.mkIdx, this]
+theorem find?_eq_findEntry?_map (m : HashMap α β) (a : α)
+    : m.find? a = (m.findEntry? a).map (·.2) := by
+  sorry
 
 theorem findEntry?_eq_some (m : HashMap α β) (a : α) (b : β)
     : m.findEntry? a = some (a, b) ↔ (∃ a', a == a' ∧ (a', b) ∈ m.toListModel) := by
   sorry
 
-theorem find?_eq (m : HashMap α β) (a : α)
-    : m.find? a = (m.findEntry? a).map (·.2) := by
-  sorry
-
-theorem toListModel_insert_perm_cons_eraseP (m : HashMap α β) (a : α) (b : β)
-    : (m.insert a b).toListModel ~ (a, b) :: m.toListModel.eraseP (·.1 == a) :=
-  sorry
-
 theorem toListModel_insert (m : HashMap α β) (a : α) (b : β)
     : (m.insert a b).toListModel ~ (a, b) :: m.toListModel.filter (·.1 != a) :=
   toListModel_eraseP_eq_toListModel_filter m ▸ toListModel_insert_perm_cons_eraseP m a b
-
-theorem toListModel_erase_perm_eraseP (m : HashMap α β) (a : α)
-    : (m.erase a).toListModel ~ m.toListModel.eraseP (·.1 == a) :=
-  sorry
 
 theorem toListModel_erase (m : HashMap α β) (a : α)
     : (m.erase a).toListModel ~ m.toListModel.filter (·.1 != a) :=
